Fixes to base case of definability
Revert [reg_offset] to a simple pattern match instead of relying on
arithmetic to keep the base case of the proof of definability working
without changes, except for the new memory invariant, which needs to be
proved.

Source/Definability.v
@@ -288,15 +288,15 @@ Section Definability.
      immediately after the back-translation counter in position 0.
      RB: TODO: Phrase in terms of [Register.to_nat]. *)
   Definition reg_offset (reg : Eregister) : Z :=
-    4 +
+    (* 4 + *)
     match reg with
-    | E_R_ONE  => 0
-    | E_R_COM  => 1
-    | E_R_AUX1 => 2
-    | E_R_AUX2 => 3
-    | E_R_RA   => 4
-    | E_R_SP   => 5
-    | E_R_ARG  => 6
+    | E_R_ONE  => 4
+    | E_R_COM  => 5
+    | E_R_AUX1 => 6
+    | E_R_AUX2 => 7
+    | E_R_RA   => 8
+    | E_R_SP   => 9
+    | E_R_ARG  => 10
     end.
 
   Lemma reg_offset_inj :
@@ -1531,6 +1531,19 @@ Section Definability.
       auto.
     Qed.
 
+    (* TODO: Relocate *)
+    Remark reg_offset0 r : reg_offset r <> 0%Z.
+    Proof.
+      destruct r; discriminate.
+    Qed.
+
+    Remark pointer_reg_offset0
+           (P : Permission.id) (C : Component.id) (b : Block.id) r :
+      (P, C, b, reg_offset r) <> (P, C, b, 0%Z).
+    Proof.
+      injection. apply reg_offset0.
+    Qed.
+
     (* TODO: [DynShare] Trace relation should appear here too!
 
        Well-bracketedness, etc., probably need to be rewritten to operate "in
@@ -1590,7 +1603,6 @@ Section Definability.
                     (Source.prepare_buffers p)
                     (Permission.data, Component.main, Block.local, reg_offset E_R_ONE)
                     Undef Undef) as [mem1 Hmem1]; eauto.
-(* FIXME
         destruct (Memory.store_after_load
                     mem1
                     (Permission.data, Component.main, Block.local, reg_offset E_R_AUX1)
@@ -1649,11 +1661,13 @@ Section Definability.
         split; [| split; [| split]].
         + rewrite /CS.initial_machine_state /Source.prog_main
                   find_procedures_of_trace_main.
+(* FIXME
           repeat (take_step; eauto). instantiate (1 := Int 1%Z).
           admit.
           repeat (take_step; eauto).
-          now apply star_refl.
-
+          (* now apply star_refl. *)
+*)
+          admit.
         + reflexivity.
         + now do 2 constructor.
         + econstructor; eauto.
@@ -1696,8 +1710,6 @@ Section Definability.
                   all: admit.
             -- by move=> [].
           * unfold valid_procedure. now auto.
-*)
-        admit.
     - (* Inductive step. *)
       rewrite -catA => Et.
       assert (wf_int_pref' : well_formed_intermediate_prefix (prefix ++ [:: e])).
